Automata/Addition.lean
@@ -4,13 +4,13 @@ import Automata.DFA
 import Automata.NFA
 import Mathlib.Data.Nat.Digits
 
-def addBase (k: ℕ) : DFA (Fin 3 → Fin k) (Fin 3) := {
+def addBase (b m: ℕ) (i j k : Fin m): DFA (Fin m → Fin (b+2)) (Fin 3) := {
   transition := fun f s => match s with
-    | 0 => if (f 0).val + f 1 == f 2 then 0 else
-      if (f 0).val + f 1 + 1 == f 2 then 1
+    | 0 => if (f i).val + f j == f k then 0 else
+      if (f i).val + f j + 1 == f k then 1
       else 2
-    | 1 => if (f 0).val + f 1 + 1 == f 2 + k then 1 else
-      if (f 0).val + f 1 == f 2 + k then 0
+    | 1 => if (f i).val + f j + 1 == f k + b then 1 else
+      if (f i).val + f j == f k + b then 0
       else 2
     | 2 => 2
   start := 0
